example/Escrow.thy
@@ -5,35 +5,39 @@ imports
 begin
 (*
 pragma solidity ^0.4.0;
-contract EscrowWallet {
+contract Escrow {
 
-    address from;
-    address to;
-    address owner;
+    address buyer;
+    address seller;
+    address arbiter;
+    uint256 amount;
 
-    function EscrowWallet(address _from, address _to) public {
-            from = _from;
-            to = _to;
-            owner = msg.sender;
+    function Escrow(address _buyer, address _seller, uint256 _amount) public {
+            require (amount > 0 && _buyer != 0 && _seller != 0);
+            buyer = _buyer;
+            seller = _seller;
+            arbiter = msg.sender;
+            amount = _amount;
     }
 
     function addfund() payable public  {
-        require (msg.value > 0 && msg.sender == from);
+        require (amount > 0 && msg.value == amount && msg.sender == buyer);
+        amount = 0;
     }
 
     function refund() public {
-        require (msg.sender == owner);
-        selfdestruct(from);
+        require (amount == 0 && msg.sender == arbiter);
+        selfdestruct(buyer);
     }
 
     function pay() public {
-        require (msg.sender == owner);
-        selfdestruct(to);
+        require (amount == 0 && msg.sender == arbiter);
+        selfdestruct(seller);
     }
 }
 
 Compiled with:
- solc --optimize --overwrite -o escrow --bin-runtime --asm --hashes escrow.sol
+ solc --optimize --overwrite -o escrow2 --bin-runtime --asm --hashes escrow2.sol
 
 8f9595d4: addfund()
 1b9265b8: pay()
@@ -41,147 +45,167 @@ Compiled with:
 
 
 *)
-value"(parse_bytecode ''6060604052600436106100565763ffffffff7c01000000000000000000000000000000000000000000000000000000006000350416631b9265b8811461005b578063590e1ae3146100705780638f9595d414610083575b600080fd5b341561006657600080fd5b61006e61008b565b005b341561007b57600080fd5b61006e6100ce565b61006e610111565b6002543373ffffffffffffffffffffffffffffffffffffffff9081169116146100b357600080fd5b60015473ffffffffffffffffffffffffffffffffffffffff16ff5b6002543373ffffffffffffffffffffffffffffffffffffffff9081169116146100f657600080fd5b60005473ffffffffffffffffffffffffffffffffffffffff16ff5b60003411801561013c57506000543373ffffffffffffffffffffffffffffffffffffffff9081169116145b151561014757600080fd5b5600a165627a7a7230582042e50839f6b362829e3a909e36d9b74b844a99ec99d3c9b1d94feddfa1215f1b0029'')"
+value"(parse_bytecode ''606060405263ffffffff7c01000000000000000000000000000000000000000000000000000000006000350416631b9265b88114610052578063590e1ae3146100675780638f9595d41461007a57600080fd5b341561005d57600080fd5b610065610082565b005b341561007257600080fd5b6100656100d3565b610065610124565b6003541580156100ad57506002543373ffffffffffffffffffffffffffffffffffffffff9081169116145b15156100b857600080fd5b60015473ffffffffffffffffffffffffffffffffffffffff16ff5b6003541580156100fe57506002543373ffffffffffffffffffffffffffffffffffffffff9081169116145b151561010957600080fd5b60005473ffffffffffffffffffffffffffffffffffffffff16ff5b6000600354118015610137575060035434145b801561015e57506000543373ffffffffffffffffffffffffffffffffffffffff9081169116145b151561016957600080fd5b60006003555600a165627a7a7230582029f2f38b5b84c1c55e91aaca3d9362e635c88ad7e3be217a7183f3cccee1aed40029'')"
 
 definition insts_ex where
-"insts_ex == [Stack (PUSH_N [0x60]), Stack (PUSH_N [0x40]), Memory MSTORE, Stack (PUSH_N [4]), Info CALLDATASIZE,
-  Arith inst_LT, Stack (PUSH_N [0, 0x56]), Pc JUMPI, Stack (PUSH_N [0xFF, 0xFF, 0xFF, 0xFF]),
+"insts_ex == [Stack (PUSH_N [0x60]), Stack (PUSH_N [0x40]), Memory MSTORE, Stack (PUSH_N [0xFF, 0xFF, 0xFF, 0xFF]),
   Stack (PUSH_N [1, 0, 0, 0, 0, 0, 0, 0, 0, 0, 0, 0, 0, 0, 0, 0, 0, 0, 0, 0, 0, 0, 0, 0, 0, 0, 0, 0, 0]),
-  Stack (PUSH_N [0]), Stack CALLDATALOAD, Arith DIV, Bits inst_AND, Stack (PUSH_N [0x1B, 0x92, 0x65, 0xB8]),
-  Dup 1, Arith inst_EQ, Stack (PUSH_N [0, 0x5B]), Pc JUMPI, Dup 0, Stack (PUSH_N [0x59, 0xE, 0x1A, 0xE3]),
-  Arith inst_EQ, Stack (PUSH_N [0, 0x70]), Pc JUMPI, Dup 0, Stack (PUSH_N [0x8F, 0x95, 0x95, 0xD4]),
-  Arith inst_EQ, Stack (PUSH_N [0, 0x83]), Pc JUMPI, Pc JUMPDEST, Stack (PUSH_N [0]), Dup 0, Unknown 0xFD,
-  Pc JUMPDEST, Info CALLVALUE, Arith ISZERO, Stack (PUSH_N [0, 0x66]), Pc JUMPI, Stack (PUSH_N [0]), Dup 0,
-  Unknown 0xFD, Pc JUMPDEST, Stack (PUSH_N [0, 0x6E]), Stack (PUSH_N [0, 0x8B]), Pc JUMP, Pc JUMPDEST,
-  Misc STOP, Pc JUMPDEST, Info CALLVALUE, Arith ISZERO, Stack (PUSH_N [0, 0x7B]), Pc JUMPI,
-  Stack (PUSH_N [0]), Dup 0, Unknown 0xFD, Pc JUMPDEST, Stack (PUSH_N [0, 0x6E]), Stack (PUSH_N [0, 0xCE]),
-  Pc JUMP, Pc JUMPDEST, Stack (PUSH_N [0, 0x6E]), Stack (PUSH_N [1, 0x11]), Pc JUMP, Pc JUMPDEST,
+  Stack (PUSH_N [0]), Stack CALLDATALOAD, Arith DIV, Bits inst_AND,
+  Stack (PUSH_N [0x1B, 0x92, 0x65, 0xB8]), Dup 1, Arith inst_EQ, Stack (PUSH_N [0, 0x52]), Pc JUMPI, Dup 0,
+  Stack (PUSH_N [0x59, 0xE, 0x1A, 0xE3]), Arith inst_EQ, Stack (PUSH_N [0, 0x67]), Pc JUMPI, Dup 0,
+  Stack (PUSH_N [0x8F, 0x95, 0x95, 0xD4]), Arith inst_EQ, Stack (PUSH_N [0, 0x7A]), Pc JUMPI,
+  Stack (PUSH_N [0]), Dup 0, Unknown 0xFD, Pc JUMPDEST, Info CALLVALUE, Arith ISZERO,
+  Stack (PUSH_N [0, 0x5D]), Pc JUMPI, Stack (PUSH_N [0]), Dup 0, Unknown 0xFD, Pc JUMPDEST,
+  Stack (PUSH_N [0, 0x65]), Stack (PUSH_N [0, 0x82]), Pc JUMP, Pc JUMPDEST, Misc STOP, Pc JUMPDEST,
+  Info CALLVALUE, Arith ISZERO, Stack (PUSH_N [0, 0x72]), Pc JUMPI, Stack (PUSH_N [0]), Dup 0,
+  Unknown 0xFD, Pc JUMPDEST, Stack (PUSH_N [0, 0x65]), Stack (PUSH_N [0, 0xD3]), Pc JUMP, Pc JUMPDEST,
+  Stack (PUSH_N [0, 0x65]), Stack (PUSH_N [1, 0x24]), Pc JUMP, Pc JUMPDEST, Stack (PUSH_N [3]),
+  Storage SLOAD, Arith ISZERO, Dup 0, Arith ISZERO, Stack (PUSH_N [0, 0xAD]), Pc JUMPI, Stack POP,
   Stack (PUSH_N [2]), Storage SLOAD, Info CALLER,
   Stack (PUSH_N
           [0xFF, 0xFF, 0xFF, 0xFF, 0xFF, 0xFF, 0xFF, 0xFF, 0xFF, 0xFF, 0xFF, 0xFF, 0xFF, 0xFF, 0xFF, 0xFF,
            0xFF, 0xFF, 0xFF, 0xFF]),
-  Swap 0, Dup 1, Bits inst_AND, Swap 1, Bits inst_AND, Arith inst_EQ, Stack (PUSH_N [0, 0xB3]), Pc JUMPI,
-  Stack (PUSH_N [0]), Dup 0, Unknown 0xFD, Pc JUMPDEST, Stack (PUSH_N [1]), Storage SLOAD,
+  Swap 0, Dup 1, Bits inst_AND, Swap 1, Bits inst_AND, Arith inst_EQ, Pc JUMPDEST, Arith ISZERO,
+  Arith ISZERO, Stack (PUSH_N [0, 0xB8]), Pc JUMPI, Stack (PUSH_N [0]), Dup 0, Unknown 0xFD, Pc JUMPDEST,
+  Stack (PUSH_N [1]), Storage SLOAD,
   Stack (PUSH_N
           [0xFF, 0xFF, 0xFF, 0xFF, 0xFF, 0xFF, 0xFF, 0xFF, 0xFF, 0xFF, 0xFF, 0xFF, 0xFF, 0xFF, 0xFF, 0xFF,
            0xFF, 0xFF, 0xFF, 0xFF]),
-  Bits inst_AND, Misc SUICIDE, Pc JUMPDEST, Stack (PUSH_N [2]), Storage SLOAD, Info CALLER,
+  Bits inst_AND, Misc SUICIDE, Pc JUMPDEST, Stack (PUSH_N [3]), Storage SLOAD, Arith ISZERO, Dup 0,
+  Arith ISZERO, Stack (PUSH_N [0, 0xFE]), Pc JUMPI, Stack POP, Stack (PUSH_N [2]), Storage SLOAD,
+  Info CALLER,
   Stack (PUSH_N
           [0xFF, 0xFF, 0xFF, 0xFF, 0xFF, 0xFF, 0xFF, 0xFF, 0xFF, 0xFF, 0xFF, 0xFF, 0xFF, 0xFF, 0xFF, 0xFF,
            0xFF, 0xFF, 0xFF, 0xFF]),
-  Swap 0, Dup 1, Bits inst_AND, Swap 1, Bits inst_AND, Arith inst_EQ, Stack (PUSH_N [0, 0xF6]), Pc JUMPI,
-  Stack (PUSH_N [0]), Dup 0, Unknown 0xFD, Pc JUMPDEST, Stack (PUSH_N [0]), Storage SLOAD,
+  Swap 0, Dup 1, Bits inst_AND, Swap 1, Bits inst_AND, Arith inst_EQ, Pc JUMPDEST, Arith ISZERO,
+  Arith ISZERO, Stack (PUSH_N [1, 9]), Pc JUMPI, Stack (PUSH_N [0]), Dup 0, Unknown 0xFD, Pc JUMPDEST,
+  Stack (PUSH_N [0]), Storage SLOAD,
   Stack (PUSH_N
           [0xFF, 0xFF, 0xFF, 0xFF, 0xFF, 0xFF, 0xFF, 0xFF, 0xFF, 0xFF, 0xFF, 0xFF, 0xFF, 0xFF, 0xFF, 0xFF,
            0xFF, 0xFF, 0xFF, 0xFF]),
-  Bits inst_AND, Misc SUICIDE, Pc JUMPDEST, Stack (PUSH_N [0]), Info CALLVALUE, Arith inst_GT, Dup 0,
-  Arith ISZERO, Stack (PUSH_N [1, 0x3C]), Pc JUMPI, Stack POP, Stack (PUSH_N [0]), Storage SLOAD, Info CALLER,
+  Bits inst_AND, Misc SUICIDE, Pc JUMPDEST, Stack (PUSH_N [0]), Stack (PUSH_N [3]), Storage SLOAD,
+  Arith inst_GT, Dup 0, Arith ISZERO, Stack (PUSH_N [1, 0x37]), Pc JUMPI, Stack POP, Stack (PUSH_N [3]),
+  Storage SLOAD, Info CALLVALUE, Arith inst_EQ, Pc JUMPDEST, Dup 0, Arith ISZERO, Stack (PUSH_N [1, 0x5E]),
+  Pc JUMPI, Stack POP, Stack (PUSH_N [0]), Storage SLOAD, Info CALLER,
   Stack (PUSH_N
           [0xFF, 0xFF, 0xFF, 0xFF, 0xFF, 0xFF, 0xFF, 0xFF, 0xFF, 0xFF, 0xFF, 0xFF, 0xFF, 0xFF, 0xFF, 0xFF,
            0xFF, 0xFF, 0xFF, 0xFF]),
-  Swap 0, Dup 1, Bits inst_AND, Swap 1, Bits inst_AND, Arith inst_EQ, Pc JUMPDEST, Arith ISZERO, Arith ISZERO,
-  Stack (PUSH_N [1, 0x47]), Pc JUMPI, Stack (PUSH_N [0]), Dup 0, Unknown 0xFD, Pc JUMPDEST, Pc JUMP,
-  Misc STOP, Log LOG1, Stack (PUSH_N [0x62, 0x7A, 0x7A, 0x72, 0x30, 0x58]), Arith SHA3, Info TIMESTAMP,
-  Unknown 0xE5, Arith ADDMOD, Memory CODECOPY, Unknown 0xF6, Unknown 0xB3, Stack (PUSH_N [0x82, 0x9E, 0x3A]),
-  Swap 0, Swap 0xE, Info CALLDATASIZE, Unknown 0xD9, Unknown 0xB7, Unknown 0x4B, Dup 4, Unknown 0x4A, Swap 9,
-  Unknown 0xEC, Swap 9, Unknown 0xD3, Unknown 0xC9, Unknown 0xB1, Unknown 0xD9, Unknown 0x4F, Unknown 0xED,
-  Unknown 0xDF, Log LOG1, Unknown 0x21, Unknown 0x5F, Unknown 0x1B, Misc STOP, Unknown 0x29]"
+  Swap 0, Dup 1, Bits inst_AND, Swap 1, Bits inst_AND, Arith inst_EQ, Pc JUMPDEST, Arith ISZERO,
+  Arith ISZERO, Stack (PUSH_N [1, 0x69]), Pc JUMPI, Stack (PUSH_N [0]), Dup 0, Unknown 0xFD, Pc JUMPDEST,
+  Stack (PUSH_N [0]), Stack (PUSH_N [3]), Storage SSTORE, Pc JUMP, Misc STOP, Log LOG1,
+  Stack (PUSH_N [0x62, 0x7A, 0x7A, 0x72, 0x30, 0x58]), Arith SHA3, Unknown 0x29, Misc CALLCODE,
+  Misc RETURN, Dup 0xB, Pc JUMPDEST, Dup 4, Unknown 0xC1, Unknown 0xC5, Unknown 0x5E, Swap 1, Unknown 0xAA,
+  Unknown 0xCA, Unknown 0x3D, Swap 3, Stack (PUSH_N [0xE6, 0x35, 0xC8]), Dup 0xA, Unknown 0xD7,
+  Unknown 0xE3, Unknown 0xBE, Unknown 0x21,
+  Stack (PUSH_N [0x71, 0x83, 0xF3, 0xCC, 0xCE, 0xE1, 0xAE, 0xD4, 0, 0x29])]"
 value "length insts_ex"
-(* 171 instructions *)
+(* 191 instructions *)
 
 lemma
- "parse_bytecode ''6060604052600436106100565763ffffffff7c01000000000000000000000000000000000000000000000000000000006000350416631b9265b8811461005b578063590e1ae3146100705780638f9595d414610083575b600080fd5b341561006657600080fd5b61006e61008b565b005b341561007b57600080fd5b61006e6100ce565b61006e610111565b6002543373ffffffffffffffffffffffffffffffffffffffff9081169116146100b357600080fd5b60015473ffffffffffffffffffffffffffffffffffffffff16ff5b6002543373ffffffffffffffffffffffffffffffffffffffff9081169116146100f657600080fd5b60005473ffffffffffffffffffffffffffffffffffffffff16ff5b60003411801561013c57506000543373ffffffffffffffffffffffffffffffffffffffff9081169116145b151561014757600080fd5b5600a165627a7a7230582042e50839f6b362829e3a909e36d9b74b844a99ec99d3c9b1d94feddfa1215f1b0029'' = insts_ex"
+ "parse_bytecode ''606060405263ffffffff7c01000000000000000000000000000000000000000000000000000000006000350416631b9265b88114610052578063590e1ae3146100675780638f9595d41461007a57600080fd5b341561005d57600080fd5b610065610082565b005b341561007257600080fd5b6100656100d3565b610065610124565b6003541580156100ad57506002543373ffffffffffffffffffffffffffffffffffffffff9081169116145b15156100b857600080fd5b60015473ffffffffffffffffffffffffffffffffffffffff16ff5b6003541580156100fe57506002543373ffffffffffffffffffffffffffffffffffffffff9081169116145b151561010957600080fd5b60005473ffffffffffffffffffffffffffffffffffffffff16ff5b6000600354118015610137575060035434145b801561015e57506000543373ffffffffffffffffffffffffffffffffffffffff9081169116145b151561016957600080fd5b60006003555600a165627a7a7230582029f2f38b5b84c1c55e91aaca3d9362e635c88ad7e3be217a7183f3cccee1aed40029'' = insts_ex"
   unfolding insts_ex_def
   by eval
 
 definition "blocks_escrow == build_blocks insts_ex"
 value "blocks_escrow"
 lemma blocks_escrow_simp:
- "blocks_escrow = [(0, [(0, Stack (PUSH_N [0x60])), (2, Stack (PUSH_N [0x40])), (4, Memory MSTORE), (5, Stack (PUSH_N [4])),
-       (7, Info CALLDATASIZE), (8, Arith inst_LT), (9, Stack (PUSH_N [0, 0x56]))],
+ "blocks_escrow = [(0, [(0, Stack (PUSH_N [0x60])), (2, Stack (PUSH_N [0x40])), (4, Memory MSTORE),
+       (5, Stack (PUSH_N [0xFF, 0xFF, 0xFF, 0xFF])),
+       (10, Stack (PUSH_N
+                    [1, 0, 0, 0, 0, 0, 0, 0, 0, 0, 0, 0, 0, 0, 0, 0, 0, 0, 0, 0, 0, 0, 0, 0, 0, 0, 0, 0,
+                     0])),
+       (40, Stack (PUSH_N [0])), (42, Stack CALLDATALOAD), (43, Arith DIV), (44, Bits inst_AND),
+       (45, Stack (PUSH_N [0x1B, 0x92, 0x65, 0xB8])), (50, Dup 1), (51, Arith inst_EQ),
+       (52, Stack (PUSH_N [0, 0x52]))],
    Jumpi),
-  (13, [(13, Stack (PUSH_N [0xFF, 0xFF, 0xFF, 0xFF])),
-        (18, Stack (PUSH_N
-                     [1, 0, 0, 0, 0, 0, 0, 0, 0, 0, 0, 0, 0, 0, 0, 0, 0, 0, 0, 0, 0, 0, 0, 0, 0, 0, 0, 0,
-                      0])),
-        (48, Stack (PUSH_N [0])), (50, Stack CALLDATALOAD), (51, Arith DIV), (52, Bits inst_AND),
-        (53, Stack (PUSH_N [0x1B, 0x92, 0x65, 0xB8])), (58, Dup 1), (59, Arith inst_EQ),
-        (60, Stack (PUSH_N [0, 0x5B]))],
+  (56, [(56, Dup 0), (57, Stack (PUSH_N [0x59, 0xE, 0x1A, 0xE3])), (62, Arith inst_EQ),
+        (63, Stack (PUSH_N [0, 0x67]))],
    Jumpi),
-  (64, [(64, Dup 0), (65, Stack (PUSH_N [0x59, 0xE, 0x1A, 0xE3])), (70, Arith inst_EQ),
-        (71, Stack (PUSH_N [0, 0x70]))],
+  (67, [(67, Dup 0), (68, Stack (PUSH_N [0x8F, 0x95, 0x95, 0xD4])), (73, Arith inst_EQ),
+        (74, Stack (PUSH_N [0, 0x7A]))],
    Jumpi),
-  (75, [(75, Dup 0), (76, Stack (PUSH_N [0x8F, 0x95, 0x95, 0xD4])), (81, Arith inst_EQ),
-        (82, Stack (PUSH_N [0, 0x83]))],
+  (78, [(78, Stack (PUSH_N [0])), (80, Dup 0), (81, Unknown 0xFD)], Terminal),
+  (82, [(82, Pc JUMPDEST), (83, Info CALLVALUE), (84, Arith ISZERO), (85, Stack (PUSH_N [0, 0x5D]))],
    Jumpi),
-  (86, [(86, Pc JUMPDEST), (87, Stack (PUSH_N [0])), (89, Dup 0), (90, Unknown 0xFD)], Terminal),
-  (91, [(91, Pc JUMPDEST), (92, Info CALLVALUE), (93, Arith ISZERO), (94, Stack (PUSH_N [0, 0x66]))], Jumpi),
-  (98, [(98, Stack (PUSH_N [0])), (100, Dup 0), (101, Unknown 0xFD)], Terminal),
-  (102, [(102, Pc JUMPDEST), (103, Stack (PUSH_N [0, 0x6E])), (106, Stack (PUSH_N [0, 0x8B]))], Jump),
-  (110, [(110, Pc JUMPDEST), (111, Misc STOP)], Terminal),
-  (112, [(112, Pc JUMPDEST), (113, Info CALLVALUE), (114, Arith ISZERO), (115, Stack (PUSH_N [0, 0x7B]))],
+  (89, [(89, Stack (PUSH_N [0])), (91, Dup 0), (92, Unknown 0xFD)], Terminal),
+  (93, [(93, Pc JUMPDEST), (94, Stack (PUSH_N [0, 0x65])), (97, Stack (PUSH_N [0, 0x82]))], Jump),
+  (101, [(101, Pc JUMPDEST), (102, Misc STOP)], Terminal),
+  (103, [(103, Pc JUMPDEST), (104, Info CALLVALUE), (105, Arith ISZERO), (106, Stack (PUSH_N [0, 0x72]))],
    Jumpi),
-  (119, [(119, Stack (PUSH_N [0])), (121, Dup 0), (122, Unknown 0xFD)], Terminal),
-  (123, [(123, Pc JUMPDEST), (124, Stack (PUSH_N [0, 0x6E])), (127, Stack (PUSH_N [0, 0xCE]))], Jump),
-  (131, [(131, Pc JUMPDEST), (132, Stack (PUSH_N [0, 0x6E])), (135, Stack (PUSH_N [1, 0x11]))], Jump),
-  (139, [(139, Pc JUMPDEST), (140, Stack (PUSH_N [2])), (142, Storage SLOAD), (143, Info CALLER),
-         (144, Stack (PUSH_N
+  (110, [(110, Stack (PUSH_N [0])), (112, Dup 0), (113, Unknown 0xFD)], Terminal),
+  (114, [(114, Pc JUMPDEST), (115, Stack (PUSH_N [0, 0x65])), (118, Stack (PUSH_N [0, 0xD3]))], Jump),
+  (122, [(122, Pc JUMPDEST), (123, Stack (PUSH_N [0, 0x65])), (126, Stack (PUSH_N [1, 0x24]))], Jump),
+  (130, [(130, Pc JUMPDEST), (131, Stack (PUSH_N [3])), (133, Storage SLOAD), (134, Arith ISZERO),
+         (135, Dup 0), (136, Arith ISZERO), (137, Stack (PUSH_N [0, 0xAD]))],
+   Jumpi),
+  (141, [(141, Stack POP), (142, Stack (PUSH_N [2])), (144, Storage SLOAD), (145, Info CALLER),
+         (146, Stack (PUSH_N
                        [0xFF, 0xFF, 0xFF, 0xFF, 0xFF, 0xFF, 0xFF, 0xFF, 0xFF, 0xFF, 0xFF, 0xFF, 0xFF, 0xFF,
                         0xFF, 0xFF, 0xFF, 0xFF, 0xFF, 0xFF])),
-         (165, Swap 0), (166, Dup 1), (167, Bits inst_AND), (168, Swap 1), (169, Bits inst_AND),
-         (170, Arith inst_EQ), (171, Stack (PUSH_N [0, 0xB3]))],
-   Jumpi),
-  (175, [(175, Stack (PUSH_N [0])), (177, Dup 0), (178, Unknown 0xFD)], Terminal),
-  (179, [(179, Pc JUMPDEST), (180, Stack (PUSH_N [1])), (182, Storage SLOAD),
-         (183, Stack (PUSH_N
-                       [0xFF, 0xFF, 0xFF, 0xFF, 0xFF, 0xFF, 0xFF, 0xFF, 0xFF, 0xFF, 0xFF, 0xFF, 0xFF, 0xFF,
-                        0xFF, 0xFF, 0xFF, 0xFF, 0xFF, 0xFF])),
-         (204, Bits inst_AND), (205, Misc SUICIDE)],
-   Terminal),
-  (206, [(206, Pc JUMPDEST), (207, Stack (PUSH_N [2])), (209, Storage SLOAD), (210, Info CALLER),
-         (211, Stack (PUSH_N
-                       [0xFF, 0xFF, 0xFF, 0xFF, 0xFF, 0xFF, 0xFF, 0xFF, 0xFF, 0xFF, 0xFF, 0xFF, 0xFF, 0xFF,
-                        0xFF, 0xFF, 0xFF, 0xFF, 0xFF, 0xFF])),
-         (232, Swap 0), (233, Dup 1), (234, Bits inst_AND), (235, Swap 1), (236, Bits inst_AND),
-         (237, Arith inst_EQ), (238, Stack (PUSH_N [0, 0xF6]))],
-   Jumpi),
-  (242, [(242, Stack (PUSH_N [0])), (244, Dup 0), (245, Unknown 0xFD)], Terminal),
-  (246, [(246, Pc JUMPDEST), (247, Stack (PUSH_N [0])), (249, Storage SLOAD),
-         (250, Stack (PUSH_N
-                       [0xFF, 0xFF, 0xFF, 0xFF, 0xFF, 0xFF, 0xFF, 0xFF, 0xFF, 0xFF, 0xFF, 0xFF, 0xFF, 0xFF,
-                        0xFF, 0xFF, 0xFF, 0xFF, 0xFF, 0xFF])),
-         (271, Bits inst_AND), (272, Misc SUICIDE)],
-   Terminal),
-  (273, [(273, Pc JUMPDEST), (274, Stack (PUSH_N [0])), (276, Info CALLVALUE), (277, Arith inst_GT),
-         (278, Dup 0), (279, Arith ISZERO), (280, Stack (PUSH_N [1, 0x3C]))],
-   Jumpi),
-  (284, [(284, Stack POP), (285, Stack (PUSH_N [0])), (287, Storage SLOAD), (288, Info CALLER),
-         (289, Stack (PUSH_N
-                       [0xFF, 0xFF, 0xFF, 0xFF, 0xFF, 0xFF, 0xFF, 0xFF, 0xFF, 0xFF, 0xFF, 0xFF, 0xFF, 0xFF,
-                        0xFF, 0xFF, 0xFF, 0xFF, 0xFF, 0xFF])),
-         (310, Swap 0), (311, Dup 1), (312, Bits inst_AND), (313, Swap 1), (314, Bits inst_AND),
-         (315, Arith inst_EQ)],
+         (167, Swap 0), (168, Dup 1), (169, Bits inst_AND), (170, Swap 1), (171, Bits inst_AND),
+         (172, Arith inst_EQ)],
    Next),
-  (316, [(316, Pc JUMPDEST), (317, Arith ISZERO), (318, Arith ISZERO), (319, Stack (PUSH_N [1, 0x47]))],
+  (173, [(173, Pc JUMPDEST), (174, Arith ISZERO), (175, Arith ISZERO), (176, Stack (PUSH_N [0, 0xB8]))],
    Jumpi),
-  (323, [(323, Stack (PUSH_N [0])), (325, Dup 0), (326, Unknown 0xFD)], Terminal),
-  (327, [(327, Pc JUMPDEST)], Jump), (329, [(329, Misc STOP)], Terminal),
-  (330, [(330, Log LOG1), (331, Stack (PUSH_N [0x62, 0x7A, 0x7A, 0x72, 0x30, 0x58])), (338, Arith SHA3),
-         (339, Info TIMESTAMP), (340, Unknown 0xE5)],
+  (180, [(180, Stack (PUSH_N [0])), (182, Dup 0), (183, Unknown 0xFD)], Terminal),
+  (184, [(184, Pc JUMPDEST), (185, Stack (PUSH_N [1])), (187, Storage SLOAD),
+         (188, Stack (PUSH_N
+                       [0xFF, 0xFF, 0xFF, 0xFF, 0xFF, 0xFF, 0xFF, 0xFF, 0xFF, 0xFF, 0xFF, 0xFF, 0xFF, 0xFF,
+                        0xFF, 0xFF, 0xFF, 0xFF, 0xFF, 0xFF])),
+         (209, Bits inst_AND), (210, Misc SUICIDE)],
    Terminal),
-  (341, [(341, Arith ADDMOD), (342, Memory CODECOPY), (343, Unknown 0xF6)], Terminal),
-  (344, [(344, Unknown 0xB3)], Terminal),
-  (345, [(345, Stack (PUSH_N [0x82, 0x9E, 0x3A])), (349, Swap 0), (350, Swap 0xE), (351, Info CALLDATASIZE),
-         (352, Unknown 0xD9)],
+  (211, [(211, Pc JUMPDEST), (212, Stack (PUSH_N [3])), (214, Storage SLOAD), (215, Arith ISZERO),
+         (216, Dup 0), (217, Arith ISZERO), (218, Stack (PUSH_N [0, 0xFE]))],
+   Jumpi),
+  (222, [(222, Stack POP), (223, Stack (PUSH_N [2])), (225, Storage SLOAD), (226, Info CALLER),
+         (227, Stack (PUSH_N
+                       [0xFF, 0xFF, 0xFF, 0xFF, 0xFF, 0xFF, 0xFF, 0xFF, 0xFF, 0xFF, 0xFF, 0xFF, 0xFF, 0xFF,
+                        0xFF, 0xFF, 0xFF, 0xFF, 0xFF, 0xFF])),
+         (248, Swap 0), (249, Dup 1), (250, Bits inst_AND), (251, Swap 1), (252, Bits inst_AND),
+         (253, Arith inst_EQ)],
+   Next),
+  (254, [(254, Pc JUMPDEST), (255, Arith ISZERO), (256, Arith ISZERO), (257, Stack (PUSH_N [1, 9]))],
+   Jumpi),
+  (261, [(261, Stack (PUSH_N [0])), (263, Dup 0), (264, Unknown 0xFD)], Terminal),
+  (265, [(265, Pc JUMPDEST), (266, Stack (PUSH_N [0])), (268, Storage SLOAD),
+         (269, Stack (PUSH_N
+                       [0xFF, 0xFF, 0xFF, 0xFF, 0xFF, 0xFF, 0xFF, 0xFF, 0xFF, 0xFF, 0xFF, 0xFF, 0xFF, 0xFF,
+                        0xFF, 0xFF, 0xFF, 0xFF, 0xFF, 0xFF])),
+         (290, Bits inst_AND), (291, Misc SUICIDE)],
    Terminal),
-  (353, [(353, Unknown 0xB7)], Terminal), (354, [(354, Unknown 0x4B)], Terminal),
-  (355, [(355, Dup 4), (356, Unknown 0x4A)], Terminal), (357, [(357, Swap 9), (358, Unknown 0xEC)], Terminal),
-  (359, [(359, Swap 9), (360, Unknown 0xD3)], Terminal), (361, [(361, Unknown 0xC9)], Terminal),
-  (362, [(362, Unknown 0xB1)], Terminal), (363, [(363, Unknown 0xD9)], Terminal),
-  (364, [(364, Unknown 0x4F)], Terminal), (365, [(365, Unknown 0xED)], Terminal),
-  (366, [(366, Unknown 0xDF)], Terminal), (367, [(367, Log LOG1), (368, Unknown 0x21)], Terminal),
-  (369, [(369, Unknown 0x5F)], Terminal), (370, [(370, Unknown 0x1B)], Terminal),
-  (371, [(371, Misc STOP)], Terminal), (372, [(372, Unknown 0x29)], Terminal)]"
+  (292, [(292, Pc JUMPDEST), (293, Stack (PUSH_N [0])), (295, Stack (PUSH_N [3])), (297, Storage SLOAD),
+         (298, Arith inst_GT), (299, Dup 0), (300, Arith ISZERO), (301, Stack (PUSH_N [1, 0x37]))],
+   Jumpi),
+  (305, [(305, Stack POP), (306, Stack (PUSH_N [3])), (308, Storage SLOAD), (309, Info CALLVALUE),
+         (310, Arith inst_EQ)],
+   Next),
+  (311, [(311, Pc JUMPDEST), (312, Dup 0), (313, Arith ISZERO), (314, Stack (PUSH_N [1, 0x5E]))], Jumpi),
+  (318, [(318, Stack POP), (319, Stack (PUSH_N [0])), (321, Storage SLOAD), (322, Info CALLER),
+         (323, Stack (PUSH_N
+                       [0xFF, 0xFF, 0xFF, 0xFF, 0xFF, 0xFF, 0xFF, 0xFF, 0xFF, 0xFF, 0xFF, 0xFF, 0xFF, 0xFF,
+                        0xFF, 0xFF, 0xFF, 0xFF, 0xFF, 0xFF])),
+         (344, Swap 0), (345, Dup 1), (346, Bits inst_AND), (347, Swap 1), (348, Bits inst_AND),
+         (349, Arith inst_EQ)],
+   Next),
+  (350, [(350, Pc JUMPDEST), (351, Arith ISZERO), (352, Arith ISZERO), (353, Stack (PUSH_N [1, 0x69]))],
+   Jumpi),
+  (357, [(357, Stack (PUSH_N [0])), (359, Dup 0), (360, Unknown 0xFD)], Terminal),
+  (361, [(361, Pc JUMPDEST), (362, Stack (PUSH_N [0])), (364, Stack (PUSH_N [3])), (366, Storage SSTORE)],
+   Jump),
+  (368, [(368, Misc STOP)], Terminal),
+  (369, [(369, Log LOG1), (370, Stack (PUSH_N [0x62, 0x7A, 0x7A, 0x72, 0x30, 0x58])), (377, Arith SHA3),
+         (378, Unknown 0x29)],
+   Terminal),
+  (379, [(379, Misc CALLCODE)], Terminal), (380, [(380, Misc RETURN)], Terminal),
+  (381, [(381, Dup 0xB)], Next), (382, [(382, Pc JUMPDEST), (383, Dup 4), (384, Unknown 0xC1)], Terminal),
+  (385, [(385, Unknown 0xC5)], Terminal), (386, [(386, Unknown 0x5E)], Terminal),
+  (387, [(387, Swap 1), (388, Unknown 0xAA)], Terminal), (389, [(389, Unknown 0xCA)], Terminal),
+  (390, [(390, Unknown 0x3D)], Terminal),
+  (391, [(391, Swap 3), (392, Stack (PUSH_N [0xE6, 0x35, 0xC8])), (396, Dup 0xA), (397, Unknown 0xD7)],
+   Terminal),
+  (398, [(398, Unknown 0xE3)], Terminal), (399, [(399, Unknown 0xBE)], Terminal),
+  (400, [(400, Unknown 0x21)], Terminal),
+  (401, [(401, Stack (PUSH_N [0x71, 0x83, 0xF3, 0xCC, 0xCE, 0xE1, 0xAE, 0xD4, 0, 0x29]))], Next)]"
   by eval
 
 definition addfund_hash :: "32 word"  where
@@ -193,16 +217,20 @@ definition pay_hash :: "32 word"  where
 definition refund_hash :: "32 word"  where
  "refund_hash = 0x590e1ae3"
 
-definition return_action ::"address \<Rightarrow> address \<Rightarrow> address \<Rightarrow> address \<Rightarrow> 32 word \<Rightarrow> w256 \<Rightarrow> contract_action" where
-  "return_action sender from to owner hash v = 
- (if hash = addfund_hash \<and> sender = from  \<and> v > 0 then
+definition return_action ::"address \<Rightarrow> address \<Rightarrow> address \<Rightarrow> address \<Rightarrow> w256 \<Rightarrow> 32 word \<Rightarrow> w256 \<Rightarrow> contract_action" where
+  "return_action sender buyer seller arbiter amount hash v = 
+ (if hash = addfund_hash \<and> sender = buyer  \<and> v = amount \<and> amount > 0 then
     ContractReturn []
-  else if hash = refund_hash \<and> sender = owner \<and> v = 0 then
-    ContractSuicide from
-  else if hash = pay_hash \<and> sender = owner \<and> v = 0 then
-    ContractSuicide to
+  else if hash = refund_hash \<and> sender = arbiter \<and> v = 0 \<and> amount = 0 then
+    ContractSuicide buyer
+  else if hash = pay_hash \<and> sender = arbiter \<and> v = 0 \<and> amount = 0 then
+    ContractSuicide seller
   else
     ContractFail [ShouldNotHappen])"
+
+definition return_amount ::"address \<Rightarrow> address \<Rightarrow> address  \<Rightarrow> w256 \<Rightarrow> 32 word \<Rightarrow> w256 \<Rightarrow> w256" where
+  "return_amount sender buyer seller amount hash v = 
+  (if hash = addfund_hash \<and> sender = buyer \<and> v = amount \<and> amount > 0 then 0 else amount)"
 
 context
 notes
@@ -212,7 +240,7 @@ notes
   Cmem_def[simp add]
   memory_range.simps[simp del]
  if_split[ split del ] sep_fun_simps[simp del]
-gas_value_simps[simp add] pure_emp_simps[simp add]
+gas_value_simps[simp add] gas_simps[simp] pure_emp_simps[simp add]
 evm_fun_simps[simp add] sep_lc[simp del] sep_conj_first[simp add]
 pure_false_simps[simp add] iszero_stack_def[simp add]
 word256FromNat_def[simp add]
@@ -248,8 +276,20 @@ lemma ucast_160_upto_256_eq:
   by (drule ucast_up_inj; simp)
 
 method sep_imp_solve2 uses simp =
- solves \<open>(clarsimp?, ((((sep_cancel, clarsimp?)+)|simp add:simp|rule conjI)+)[1])\<close>
- | solves \<open>(clarsimp?, ((((sep_cancel, clarsimp?)+)|simp add:simp word_rcat_simps|rule conjI)+)[1])\<close>
+   solves \<open>rule conjI; rule refl\<close>
+ | solves \<open>simp\<close>
+ | solves \<open>(clarsimp?, ((((sep_cancel, clarsimp?)+)|simp add:simp|rule conjI)+)[1])\<close>
+ | solves \<open>(clarsimp?, ((((sep_cancel, clarsimp?)+)|(clarsimp split:if_split simp: simp)|rule conjI)+)[1])\<close>
+ | solves \<open>(clarsimp split:if_splits simp:word_rcat_simps) ; sep_imp_solve2 \<close>
+
+method split_conds =
+ (split if_split_asm; clarsimp simp add: word_rcat_simps)?
+
+method block_vcg2=
+  split_conds,
+  ((blocks_rule_vcg; (rule refl)?), triple_seq_vcg),
+  (sep_imp_solve2)+,
+  (solves \<open>split_conds\<close>)?
 
 theorem verify_escrow_return:
 notes
@@ -260,246 +300,207 @@ notes
   word_bool_alg.conj.commute[simp]
   length_word_rsplit_4[simp]
   ucast_160_upto_256_eq[simp]
+  hash_diff[simp]
+  eval_bit_mask[simp]
 assumes blk_num: "bn > 2463000"
 and net: "at_least_eip150 net"
 shows
 "\<exists>r. triple net
-  (program_counter 0 ** stack_height 0 ** (sent_data (word_rsplit (hash::32 word)::byte list))
+  (program_counter 0 ** stack_height 0 ** (sent_data (word_rsplit hash::byte list))
    ** sent_value v ** caller sender ** blk_num bn **
    memory_usage 0 ** continuing ** gas_pred 100000
-   ** storage 0 (ucast from)
-   ** storage 1 (ucast to)
-   ** storage 2 (ucast owner)
-   ** account_existence from from_ex 
-   ** account_existence to to_ex 
+   ** storage 0 (ucast buyer)
+   ** storage 1 (ucast seller)
+   ** storage 2 (ucast arbiter)
+   ** storage 3 amount
+   ** account_existence buyer buyer_ex 
+   ** account_existence seller seller_ex 
    ** memory (word_rcat [64::byte]) (bytestr_to_w256 [x]) **
    memory (word_rcat [96::byte]) (bytestr_to_w256 [y]))
-  blocks_escrow (action (return_action sender from to owner hash v) ** r)"
+  blocks_escrow (action (return_action sender buyer seller arbiter amount hash v)
+                 ** storage 0 (ucast buyer)
+                 ** storage 1 (ucast seller)
+                 ** storage 2 (ucast arbiter)
+                 ** storage 3 (return_amount sender buyer seller amount hash v)** r)"
   apply (insert blk_num[simplified word_less_nat_alt] net)
   apply (simp add:blocks_escrow_simp)
-  apply(simp add: return_action_def blocks_simps triple_def )
-  apply(split if_split, rule conjI)
-   apply(rule impI, ((erule conjE)+)?, rule exI)
-   apply((block_vcg)+)[1]
-   apply (sep_imp_solve2)
-  apply(split if_split, rule conjI)
+  apply(simp add: return_action_def return_amount_def blocks_simps triple_def )
+  apply(split if_split, rule conjI)+
+   apply((rule impI)+, ((erule conjE)+)?, rule exI)
+   apply ((block_vcg2)[1])
+   apply ((block_vcg2)[1])
+   apply ((block_vcg2)[1])
+   apply ((block_vcg2)[1])
+   apply ((block_vcg2)[1])
+   apply ((block_vcg2)[1])
+   apply ((block_vcg2)[1])
+   apply ((block_vcg2)[1])
+   apply ((block_vcg2)[1])
+   apply ((block_vcg2)[1])
+   apply ((block_vcg2)[1])
+   apply ((block_vcg2)[1])
+  apply (split_conds)
+(* 1*)
+  apply (clarsimp)+
+  apply(split if_split, rule conjI)+
+  apply(safe; clarsimp)
+  apply( clarsimp)
+  apply(rule exI)
+   apply ((block_vcg2)[1])
+   apply ((block_vcg2)[1])
+   apply ((block_vcg2)[1])
+   apply ((block_vcg2)[1])
+   apply ((block_vcg2)[1])
+   apply ((block_vcg2)[1])
+   apply ((block_vcg2)[1])
+   apply ((block_vcg2)[1])
+   apply ((block_vcg2)[1])
+   apply ((block_vcg2)[1])
+   apply (clarsimp split: if_split_asm simp: word_rcat_simps)
+  apply (clarsimp)+
+  apply(split if_split, rule conjI)+
+  apply(safe; clarsimp)
+  apply( clarsimp)
+  apply(rule exI)
+   apply ((block_vcg2)[1])
+   apply ((block_vcg2)[1])
+   apply ((block_vcg2)[1])
+   apply ((block_vcg2)[1])
+   apply ((block_vcg2)[1])
+   apply ((block_vcg2)[1])
+   apply ((block_vcg2)[1])
    apply (clarsimp)
-  apply (rule exI)
-    apply(((((blocks_rule_vcg; (rule refl)?), triple_seq_vcg)); sep_imp_solve2?)+)[1]
-   apply (sep_imp_solve2)+
-    apply(((((blocks_rule_vcg; (rule refl)?), triple_seq_vcg)); sep_imp_solve2?)+)[1]
-   apply (sep_imp_solve2)+
-   apply((block_vcg)+)[1]
-  apply (clarsimp split:if_splits simp:word_rcat_simps bin_cat_def hash_diff)
-   apply(((((blocks_rule_vcg; (rule refl)?), triple_seq_vcg)); sep_imp_solve2?)+)[1]
-   apply (sep_imp_solve2)+
-  apply (clarsimp split:if_splits simp:word_rcat_simps bin_cat_def hash_diff)
-   apply(((((blocks_rule_vcg; (rule refl)?), triple_seq_vcg)); sep_imp_solve2?)+)[1]
-   apply (sep_imp_solve2)+
-   apply (simp)
-   apply(((((blocks_rule_vcg; (rule refl)?), triple_seq_vcg)); sep_imp_solve2?)+)[1]
-   apply (sep_imp_solve2)+
-   apply(((((blocks_rule_vcg; (rule refl)?), triple_seq_vcg)); sep_imp_solve2?)+)[1]
-   apply (sep_imp_solve2|solves \<open>simp\<close>)+
-   apply(((((blocks_rule_vcg; (rule refl)?), triple_seq_vcg)); sep_imp_solve2?)+)[1]
-   apply (sep_imp_solve2|solves \<open>simp\<close>)+
-   apply (clarsimp simp add:word_rcat_simps bin_cat_def Csuicide_def)
-   apply ( solves \<open>(clarsimp?, ((((sep_cancel, clarsimp?)+)|clarsimp split: if_split |rule conjI)+)[1])\<close>)
-   apply (clarsimp split:if_splits simp:word_rcat_simps bin_cat_def hash_diff)
-   apply(((((blocks_rule_vcg; (rule refl)?), triple_seq_vcg)); sep_imp_solve2?)+)[1]
-   apply (sep_imp_solve2|solves \<open>simp\<close>)+
-   apply (clarsimp split:if_splits simp:word_rcat_simps bin_cat_def hash_diff)
+   apply (rule conjI)
+   apply (clarsimp simp: word_rcat_simps)
+ (* write simp rules to put stack in first pos *)
+  apply (sep_select 6)
+   apply (sep_cancel)+
+   apply (clarsimp split: if_split simp: word_rcat_simps)
+   apply (split_conds)
+   apply (sep_cancel)+
+   apply ((block_vcg2)[1])
+   apply ((block_vcg2)[1])
+   apply (split_conds)
 (*1*)
-  apply(split if_split, rule conjI)
-  apply (clarsimp)
-  apply (rule exI)
-   apply(((((blocks_rule_vcg; (rule refl)?), triple_seq_vcg)); sep_imp_solve2?)+)[1]
-   apply (sep_imp_solve2|solves \<open>simp\<close>)+
-  apply(((((blocks_rule_vcg; (rule refl)?), triple_seq_vcg)); sep_imp_solve2?)+)[1]
-  apply (sep_imp_solve2|solves \<open>simp\<close>)+
-  apply (clarsimp split:if_splits simp:word_rcat_simps bin_cat_def hash_diff)
-  apply(((((blocks_rule_vcg; (rule refl)?), triple_seq_vcg)); sep_imp_solve2?)+)[1]
-  apply (sep_imp_solve2|solves \<open>simp\<close>)+
-  apply(((((blocks_rule_vcg; (rule refl)?), triple_seq_vcg)); sep_imp_solve2?)+)[1]
-  apply (sep_imp_solve2|solves \<open>simp\<close>)+
-  apply(((((blocks_rule_vcg; (rule refl)?), triple_seq_vcg)); sep_imp_solve2?)+)[1]
-  apply (sep_imp_solve2|solves \<open>simp\<close>)+
-  apply(((((blocks_rule_vcg; (rule refl)?), triple_seq_vcg)); sep_imp_solve2?)+)[1]
-  apply (sep_imp_solve2|solves \<open>simp\<close>)+
-  apply (clarsimp simp add:word_rcat_simps bin_cat_def Csuicide_def)
-  apply ( solves \<open>(clarsimp?, ((((sep_cancel, clarsimp?)+)|clarsimp split: if_split |rule conjI)+)[1])\<close>)
-  apply (clarsimp)
-  apply (clarsimp)
-  apply (clarsimp split:if_splits simp:word_rcat_simps bin_cat_def hash_diff Csuicide_def)
-(*1*)
-  apply (clarsimp)
+  apply (clarsimp split: if_split )
+  apply (rule conjI; clarsimp)
   apply (case_tac " hash = pay_hash"; clarsimp)
-  apply (case_tac "v \<noteq> 0"; clarsimp)
-  apply (rule exI)
-  apply(((((blocks_rule_vcg; (rule refl)?), triple_seq_vcg)); sep_imp_solve2?)+)[1]
-  apply (sep_imp_solve2|solves \<open>simp\<close>)+
-  apply(((((blocks_rule_vcg; (rule refl)?), triple_seq_vcg)); sep_imp_solve2?)+)[1]
-  apply (sep_imp_solve2|solves \<open>simp\<close>)+
-  apply (clarsimp split: if_split_asm simp:word_rcat_simps bin_cat_def hash_diff)
-  apply(((((blocks_rule_vcg; (rule refl)?), triple_seq_vcg)); sep_imp_solve2?)+)[1]
-  apply (sep_imp_solve2|solves \<open>simp\<close>)+
-  apply(((((blocks_rule_vcg; (rule refl)?), triple_seq_vcg)); sep_imp_solve2?)+)[1]
-  apply (sep_imp_solve2|solves \<open>simp\<close>)+
-  apply (clarsimp split: if_split_asm simp:word_rcat_simps bin_cat_def hash_diff)
-  (*2*)
-  apply (rule exI)
-  apply(((((blocks_rule_vcg; (rule refl)?), triple_seq_vcg)); sep_imp_solve2?)+)[1]
-  apply (sep_imp_solve2|solves \<open>simp\<close>)+
-  apply(((((blocks_rule_vcg; (rule refl)?), triple_seq_vcg)); sep_imp_solve2?)+)[1]
-  apply (sep_imp_solve2|solves \<open>simp\<close>)+
-  apply (clarsimp split: if_split_asm simp:word_rcat_simps bin_cat_def hash_diff)
-  apply(((((blocks_rule_vcg; (rule refl)?), triple_seq_vcg)); sep_imp_solve2?)+)[1]
-  apply (sep_imp_solve2|solves \<open>simp\<close>)+
-  apply(((((blocks_rule_vcg; (rule refl)?), triple_seq_vcg)); sep_imp_solve2?)+)[1]
-  apply (sep_imp_solve2|solves \<open>simp\<close>)+
-  apply(((((blocks_rule_vcg; (rule refl)?), triple_seq_vcg)); sep_imp_solve2?)+)[1]
-  apply (sep_imp_solve2|solves \<open>simp\<close>)+
-  apply (clarsimp split: if_split_asm simp:word_rcat_simps bin_cat_def hash_diff)
-  apply (clarsimp split: if_split_asm simp:word_rcat_simps bin_cat_def hash_diff)
-  apply(((((blocks_rule_vcg; (rule refl)?), triple_seq_vcg)); sep_imp_solve2?)+)[1]
-  apply (sep_imp_solve2|solves \<open>simp\<close>)+
-  apply (clarsimp split: if_split_asm simp:word_rcat_simps bin_cat_def hash_diff)
+  apply (case_tac "v \<noteq> 0")
+   apply (rule exI)
+   apply ((block_vcg2)[1])
+   apply ((block_vcg2)[1])
+   apply ((block_vcg2)[1])
+   apply (split_conds)
+  apply (case_tac "amount \<noteq> 0"; clarsimp)
+  apply(rule exI)
+   apply ((block_vcg2)[1])
+   apply ((block_vcg2)[1])
+   apply ((block_vcg2)[1])
+   apply ((block_vcg2)[1])
+   apply ((block_vcg2)[1])
+   apply ((block_vcg2)[1])
+   apply ((block_vcg2)[1])
+   apply ((block_vcg2)[1])
+   apply (split_conds)
+  apply(rule exI)
+   apply ((block_vcg2)[1])
+   apply ((block_vcg2)[1])
+   apply ((block_vcg2)[1])
+   apply ((block_vcg2)[1])
+   apply ((block_vcg2)[1])
+   apply ((block_vcg2)[1])
+   apply ((block_vcg2)[1])
+   apply ((block_vcg2)[1])
+   apply (split_conds)
 (*1*)
   apply (case_tac " hash = refund_hash"; clarsimp)
-  apply (case_tac "v \<noteq> 0"; clarsimp)
-  apply (rule exI)
-  apply(((((blocks_rule_vcg; (rule refl)?), triple_seq_vcg)); sep_imp_solve2?)+)[1]
-  apply (sep_imp_solve2|solves \<open>simp\<close>)+
-  apply(((((blocks_rule_vcg; (rule refl)?), triple_seq_vcg)); sep_imp_solve2?)+)[1]
-  apply (sep_imp_solve2|solves \<open>simp\<close>)+
-  apply (clarsimp split: if_split_asm simp:word_rcat_simps bin_cat_def hash_diff)
-  apply(((((blocks_rule_vcg; (rule refl)?), triple_seq_vcg)); sep_imp_solve2?)+)[1]
-  apply (sep_imp_solve2|solves \<open>simp\<close>)+
-  apply(((((blocks_rule_vcg; (rule refl)?), triple_seq_vcg)); sep_imp_solve2?)+)[1]
-  apply (sep_imp_solve2|solves \<open>simp\<close>)+
-  apply (clarsimp split: if_split_asm simp:word_rcat_simps bin_cat_def hash_diff)
-  apply(((((blocks_rule_vcg; (rule refl)?), triple_seq_vcg)); sep_imp_solve2?)+)[1]
-  apply (sep_imp_solve2|solves \<open>simp\<close>)+
-  apply (clarsimp split: if_split_asm simp:word_rcat_simps bin_cat_def hash_diff)
-  (*2*)
-  apply (rule exI)
-  apply(((((blocks_rule_vcg; (rule refl)?), triple_seq_vcg)); sep_imp_solve2?)+)[1]
-  apply (sep_imp_solve2|solves \<open>simp\<close>)+
-  apply (clarsimp split: if_split_asm simp:word_rcat_simps bin_cat_def hash_diff)
-  apply(((((blocks_rule_vcg; (rule refl)?), triple_seq_vcg)); sep_imp_solve2?)+)[1]
-  apply (sep_imp_solve2|solves \<open>simp\<close>)+
-  apply (clarsimp split: if_split_asm simp:word_rcat_simps bin_cat_def hash_diff)
-  apply (clarsimp split: if_split_asm simp:word_rcat_simps bin_cat_def hash_diff)
-  apply(((((blocks_rule_vcg; (rule refl)?), triple_seq_vcg)); sep_imp_solve2?)+)[1]
-  apply (sep_imp_solve2|solves \<open>simp\<close>)+
-  apply (clarsimp split: if_split_asm simp:word_rcat_simps bin_cat_def hash_diff)
-  apply(((((blocks_rule_vcg; (rule refl)?), triple_seq_vcg)); sep_imp_solve2?)+)[1]
-  apply (sep_imp_solve2|solves \<open>simp\<close>)+
-  apply(((((blocks_rule_vcg; (rule refl)?), triple_seq_vcg)); sep_imp_solve2?)+)[1]
-  apply (sep_imp_solve2|solves \<open>simp\<close>)+
-  apply(((((blocks_rule_vcg; (rule refl)?), triple_seq_vcg)); sep_imp_solve2?)+)[1]
-  apply (sep_imp_solve2|solves \<open>simp\<close>)+
-  apply (clarsimp split: if_split_asm simp:word_rcat_simps bin_cat_def hash_diff)
-  apply (clarsimp split: if_split_asm simp:word_rcat_simps bin_cat_def hash_diff)
-  apply(((((blocks_rule_vcg; (rule refl)?), triple_seq_vcg)); sep_imp_solve2?)+)[1]
-  apply (sep_imp_solve2|solves \<open>simp\<close>)+
-  apply (clarsimp split: if_split_asm simp:word_rcat_simps bin_cat_def hash_diff)
+  apply (case_tac "v \<noteq> 0")
+   apply (rule exI)
+   apply ((block_vcg2)[1])
+   apply ((block_vcg2)[1])
+   apply ((block_vcg2)[1])
+   apply ((block_vcg2)[1])
+   apply (split_conds)
+  apply (case_tac "amount \<noteq> 0"; clarsimp)
+  apply(rule exI)
+   apply ((block_vcg2)[1])
+   apply ((block_vcg2)[1])
+   apply ((block_vcg2)[1])
+   apply ((block_vcg2)[1])
+   apply ((block_vcg2)[1])
+   apply ((block_vcg2)[1])
+   apply ((block_vcg2)[1])
+   apply ((block_vcg2)[1])
+   apply ((block_vcg2)[1])
+   apply (split_conds)
+  apply(rule exI)
+   apply ((block_vcg2)[1])
+   apply ((block_vcg2)[1])
+   apply ((block_vcg2)[1])
+   apply ((block_vcg2)[1])
+   apply ((block_vcg2)[1])
+   apply ((block_vcg2)[1])
+   apply ((block_vcg2)[1])
+   apply ((block_vcg2)[1])
+   apply ((block_vcg2)[1])
+   apply (split_conds)
 (*1*)
   apply (case_tac "hash = addfund_hash"; clarsimp)
-  apply (case_tac "v > 0")
-  apply (case_tac "sender \<noteq> from")
+  apply (case_tac "amount > 0")
+  apply (case_tac "amount \<noteq> v")
+  apply (case_tac "sender \<noteq> buyer")
   apply (rule exI)
-  apply(((((blocks_rule_vcg; (rule refl)?), triple_seq_vcg)); sep_imp_solve2?)+)[1]
-  apply (sep_imp_solve2|solves \<open>simp\<close>)+
-  apply (clarsimp split: if_split_asm simp:word_rcat_simps bin_cat_def hash_diff)
-  apply(((((blocks_rule_vcg; (rule refl)?), triple_seq_vcg)); sep_imp_solve2?)+)[1]
-  apply (sep_imp_solve2|solves \<open>simp\<close>)+
-  apply (clarsimp split: if_split_asm simp:word_rcat_simps bin_cat_def hash_diff)
-  apply (clarsimp split: if_split_asm simp:word_rcat_simps bin_cat_def hash_diff)
-  apply(((((blocks_rule_vcg; (rule refl)?), triple_seq_vcg)); sep_imp_solve2?)+)[1]
-  apply (sep_imp_solve2|solves \<open>simp\<close>)+
-  apply (clarsimp split: if_split_asm simp:word_rcat_simps bin_cat_def hash_diff)
-  apply (clarsimp split: if_split_asm simp:word_rcat_simps bin_cat_def hash_diff)
-  apply(((((blocks_rule_vcg; (rule refl)?), triple_seq_vcg)); sep_imp_solve2?)+)[1]
-  apply (sep_imp_solve2|solves \<open>simp\<close>)+
-  apply(((((blocks_rule_vcg; (rule refl)?), triple_seq_vcg)); sep_imp_solve2?)+)[1]
-  apply (sep_imp_solve2|solves \<open>simp\<close>)+
-  apply (clarsimp simp:word_rcat_simps bin_cat_def hash_diff)
-  apply (rule conjI; rule refl)
-  apply (clarsimp split: if_split_asm simp:word_rcat_simps bin_cat_def hash_diff)
-  apply(((((blocks_rule_vcg; (rule refl)?), triple_seq_vcg)); sep_imp_solve2?)+)[1]
-  apply (sep_imp_solve2|solves \<open>simp\<close>)+
-  apply (clarsimp  simp:word_rcat_simps bin_cat_def hash_diff)
-  apply (rule conjI; rule refl)
-  apply (clarsimp split: if_split_asm simp:word_rcat_simps bin_cat_def hash_diff)
-  apply (clarsimp split: if_split_asm simp:word_rcat_simps bin_cat_def hash_diff)
-  apply(((((blocks_rule_vcg; (rule refl)?), triple_seq_vcg)); sep_imp_solve2?)+)[1]
-  apply (sep_imp_solve2|solves \<open>simp\<close>)+
-  apply(((((blocks_rule_vcg; (rule refl)?), triple_seq_vcg)); sep_imp_solve2?)+)[1]
-  apply (sep_imp_solve2|solves \<open>simp\<close>)+
-  apply (clarsimp  simp:word_rcat_simps bin_cat_def hash_diff)
-  apply (rule conjI; rule refl)
-  apply (clarsimp split: if_split_asm simp:word_rcat_simps bin_cat_def hash_diff)
-  apply (clarsimp split: if_split_asm simp:word_rcat_simps bin_cat_def hash_diff)
-  apply(((((blocks_rule_vcg; (rule refl)?), triple_seq_vcg)); sep_imp_solve2?)+)[1]
-  apply (sep_imp_solve2|solves \<open>simp\<close>)+
-  apply (clarsimp split: if_split_asm simp:word_rcat_simps bin_cat_def hash_diff)
-(*3*)
-  apply blast
-(*2*)
+   apply ((block_vcg2)[1])
+   apply ((block_vcg2)[1])
+   apply ((block_vcg2)[1])
+   apply ((block_vcg2)[1])
+   apply ((block_vcg2)[1])
+   apply ((block_vcg2)[1])
+   apply ((block_vcg2)[1])
+   apply ((block_vcg2)[1])
+   apply ((block_vcg2)[1])
+  apply ((block_vcg2)[1])
+   apply (split_conds)
   apply (rule exI)
-  apply(((((blocks_rule_vcg; (rule refl)?), triple_seq_vcg)); sep_imp_solve2?)+)[1]
-  apply (sep_imp_solve2|solves \<open>simp\<close>)+
-  apply (clarsimp split: if_split_asm simp:word_rcat_simps bin_cat_def hash_diff)
-  apply(((((blocks_rule_vcg; (rule refl)?), triple_seq_vcg)); sep_imp_solve2?)+)[1]
-  apply (sep_imp_solve2|solves \<open>simp\<close>)+
-  apply (clarsimp split: if_split_asm simp:word_rcat_simps bin_cat_def hash_diff)
-  apply (clarsimp split: if_split_asm simp:word_rcat_simps bin_cat_def hash_diff)
-  apply(((((blocks_rule_vcg; (rule refl)?), triple_seq_vcg)); sep_imp_solve2?)+)[1]
-  apply (sep_imp_solve2|solves \<open>simp\<close>)+
-  apply (clarsimp split: if_split_asm simp:word_rcat_simps bin_cat_def hash_diff)
-  apply (clarsimp split: if_split_asm simp:word_rcat_simps bin_cat_def hash_diff)
-  apply(((((blocks_rule_vcg; (rule refl)?), triple_seq_vcg)); sep_imp_solve2?)+)[1]
-  apply (sep_imp_solve2|solves \<open>simp\<close>)+
-  apply (clarsimp split: if_split_asm simp:word_rcat_simps bin_cat_def hash_diff)
-  apply(((((blocks_rule_vcg; (rule refl)?), triple_seq_vcg)); sep_imp_solve2?)+)[1]
-  apply (sep_imp_solve2|solves \<open>simp\<close>)+
-    apply (clarsimp  simp:word_rcat_simps bin_cat_def hash_diff)
-  apply (rule conjI; rule refl)
-  apply(((((blocks_rule_vcg; (rule refl)?), triple_seq_vcg)); sep_imp_solve2?)+)[1]
-    apply (clarsimp  simp:word_rcat_simps bin_cat_def hash_diff)
-  apply (sep_imp_solve2|solves \<open>simp\<close>)+
-    apply (clarsimp  simp:word_rcat_simps bin_cat_def hash_diff)
-  apply (sep_imp_solve2|solves \<open>simp\<close>)+
-  apply (clarsimp  simp:word_rcat_simps bin_cat_def hash_diff)
-  apply (rule conjI; rule refl)
-  apply (clarsimp  simp:word_rcat_simps bin_cat_def hash_diff)
-  apply(((((blocks_rule_vcg; (rule refl)?), triple_seq_vcg)); sep_imp_solve2?)+)[1]
-  apply (sep_imp_solve2|solves \<open>simp\<close>)+
-  apply (clarsimp  simp:word_rcat_simps bin_cat_def hash_diff)
-  apply (rule conjI; rule refl)
-  apply (clarsimp  simp:word_rcat_simps bin_cat_def hash_diff)
-  apply(((((blocks_rule_vcg; (rule refl)?), triple_seq_vcg)); sep_imp_solve2?)+)[1]
-  apply (sep_imp_solve2|solves \<open>simp\<close>)+
-  apply (clarsimp split: if_split_asm simp:word_rcat_simps bin_cat_def hash_diff)
-(* 1 *)
+   apply ((block_vcg2)[1])
+   apply ((block_vcg2)[1])
+   apply ((block_vcg2)[1])
+   apply ((block_vcg2)[1])
+   apply ((block_vcg2)[1])
+   apply ((block_vcg2)[1])
+   apply ((block_vcg2)[1])
+   apply ((block_vcg2)[1])
+   apply ((block_vcg2)[1])
+   apply ((block_vcg2)[1])
+   apply (split_conds)
   apply (rule exI)
-  apply(((((blocks_rule_vcg; (rule refl)?), triple_seq_vcg)); sep_imp_solve2?)+)[1]
-  apply (sep_imp_solve2|solves \<open>simp\<close>)+
-  apply (clarsimp split: if_split_asm simp:word_rcat_simps bin_cat_def hash_diff)
-  apply(((((blocks_rule_vcg; (rule refl)?), triple_seq_vcg)); sep_imp_solve2?)+)[1]
-  apply (sep_imp_solve2|solves \<open>simp\<close>)+
-  apply (clarsimp split: if_split_asm simp:word_rcat_simps bin_cat_def hash_diff eval_bit_mask)
-  apply (clarsimp split: if_split_asm simp:word_rcat_simps bin_cat_def hash_diff eval_bit_mask)
-  apply(((((blocks_rule_vcg; (rule refl)?), triple_seq_vcg)); sep_imp_solve2?)+)[1]
-  apply (sep_imp_solve2|solves \<open>simp\<close>)+
-  apply (clarsimp split: if_split_asm simp:word_rcat_simps bin_cat_def hash_diff)
-  apply (clarsimp split: if_split_asm simp:word_rcat_simps bin_cat_def hash_diff)
-  apply(((((blocks_rule_vcg; (rule refl)?), triple_seq_vcg)); sep_imp_solve2?)+)[1]
-  apply (sep_imp_solve2|solves \<open>simp\<close>)+
-  apply (clarsimp split: if_split_asm simp:word_rcat_simps bin_cat_def hash_diff)
-  apply (clarsimp split: if_split_asm simp:word_rcat_simps bin_cat_def hash_diff)
-  apply(((((blocks_rule_vcg; (rule refl)?), triple_seq_vcg)); sep_imp_solve2?)+)[1]
-  apply (sep_imp_solve2|solves \<open>simp\<close>)+
+   apply ((block_vcg2)[1])
+   apply ((block_vcg2)[1])
+   apply ((block_vcg2)[1])
+   apply ((block_vcg2)[1])
+   apply ((block_vcg2)[1])
+   apply ((block_vcg2)[1])
+   apply ((block_vcg2)[1])
+   apply ((block_vcg2)[1])
+   apply ((block_vcg2)[1])
+   apply ((block_vcg2)[1])
+   apply (split_conds)
+  apply (rule exI)
+   apply ((block_vcg2)[1])
+   apply ((block_vcg2)[1])
+   apply ((block_vcg2)[1])
+   apply ((block_vcg2)[1])
+   apply ((block_vcg2)[1])
+   apply ((block_vcg2)[1])
+   apply ((block_vcg2)[1])
+   apply ((block_vcg2)[1])
+   apply ((block_vcg2)[1])
+   apply ((block_vcg2)[1])
+   apply (split_conds)
+  apply (rule exI)
+   apply ((block_vcg2)[1])
+   apply ((block_vcg2)[1])
+   apply ((block_vcg2)[1])
+   apply ((block_vcg2)[1])
   done
 end
